`xor.v`: add XOR_minus_mod instance, a right-involutive xor

theories/approxis/examples/xor.v
@@ -24,13 +24,13 @@ Class XOR_spec `{!approxisRGS Σ} `{XOR} :=
   { XOR_CORRECT_L := ∀ E K (x : Z) (y : nat)
                        (_: (0<=x)%Z)
                        (_: ((Z.to_nat x) < S Key))
-                       (_: y < S Key) e A,
+                       (_: y < S Support) e A,
       (REL (fill K (of_val #(xor_sem (Z.to_nat x) (y)))) << e @ E : A)
       -∗ REL (fill K (xor #x #y)) << e @ E : A
   ; XOR_CORRECT_R := ∀ E K (x : Z) (y : nat)
                        (_: (0<=x)%Z)
                        (_: ((Z.to_nat x) < S Key))
-                       (_: y < S Key) e A,
+                       (_: y < S Support) e A,
       (REL e << (fill K (of_val #(xor_sem (Z.to_nat x) (y)))) @ E : A)
       -∗ REL e << (fill K (xor #x #y)) @ E : A
   ; xor_correct_l : XOR_CORRECT_L
@@ -38,6 +38,9 @@ Class XOR_spec `{!approxisRGS Σ} `{XOR} :=
   ; xor_sem_typed :
     ⊢ (lrel_int_bounded 0 Key → lrel_int_bounded 0 Support → lrel_int_bounded 0 Support)%lrel
         xor xor
+    
+  ; xor_sem_inverse_r : forall (x y : nat), x < S Key →
+    y < S Support → xor_sem (xor_sem x y) y = x
   }.
 
 
@@ -185,6 +188,255 @@ Section xor_mod.
     - intros. eapply xor_mod_correct_l => //.
     - intros. eapply xor_mod_correct_r => //.
     - intros. simpl. eapply xor_mod_sem_typed.
-  Qed.
+    - intros x y. rewrite /xor_sem. simpl.
+      rewrite /xor_mod_sem. simpl.
+  Admitted. (* Do not satisfies xor_inverse_r 
+  TODO create another class `XOR_spec_inverse` ?*)
 
 End xor_mod.
+
+Section xor_minus_mod.
+  Variable bit : nat.
+  Definition Output2' := 2^bit - 1.
+  Definition Input2' := 2^bit-1.
+  Definition Key2' := 2^bit-1.
+  Notation Message2' := Output2'.
+  Notation Output2 := (S Output2').
+  Lemma Output2_pos: 0<Output2.
+  Proof. lia. Qed.
+
+  Definition xor_minus_mod : val :=
+    (λ: "x" "y", let: "diff" := "y" - "x" in
+      if: "y" < "x" then "diff" + #Output2 else "diff")%V.
+
+  Definition xor_minus_mod_sem (x y : nat) : nat :=
+    (if bool_decide (0 ≤ x) && bool_decide (x ≤ Output2')
+     then if bool_decide (0 ≤ y) && bool_decide (y ≤ Output2')
+          then if bool_decide (y < x)
+               then (Output2 + y - x)
+               else (y - x)
+          else y
+     else y).
+
+  Fact xor_minus_mod_sem_inverse_r : forall (x y : nat),
+    x < S Key2' → y < S Input2' →
+      xor_minus_mod_sem (xor_minus_mod_sem x y) y = x.
+  Proof. intros x y H1 H2.
+    rewrite /Key2' in H1.
+    rewrite /Input2' in H2.
+    assert (Hxpos : bool_decide (0 ≤ x) = true) by (apply bool_decide_eq_true; lia).
+    assert (Hypos : bool_decide (0 ≤ y) = true) by (apply bool_decide_eq_true; lia).
+    assert (Hxbound : bool_decide (x ≤ Output2') = true) by
+      (apply bool_decide_eq_true; rewrite /Output2'; lia).
+    assert (Hybound : bool_decide (y ≤ Output2') = true) by
+      (apply bool_decide_eq_true; rewrite /Output2'; lia).
+    rewrite /xor_minus_mod_sem.
+    rewrite Hxpos Hypos Hxbound Hybound. simpl.
+    destruct (bool_decide (y < x)) eqn:Hyx.
+    - apply bool_decide_eq_true in Hxpos.
+      apply bool_decide_eq_true in Hypos.
+      apply bool_decide_eq_true in Hxbound.
+      apply bool_decide_eq_true in Hybound.
+      apply bool_decide_eq_true in Hyx.
+      assert (Hboundxor : bool_decide (S (Message2' + y) - x ≤ Message2') = true).
+      { apply bool_decide_eq_true. lia. }
+      rewrite Hboundxor.
+      assert (Hxbound' : bool_decide (y < S (Message2' + y) - x) = true).
+      { apply bool_decide_eq_true. lia. }
+      rewrite Hxbound'.
+      apply bool_decide_eq_true in Hboundxor.
+      apply bool_decide_eq_true in Hxbound'.
+      lia.
+    - apply bool_decide_eq_true in Hxpos.
+      apply bool_decide_eq_true in Hypos.
+      apply bool_decide_eq_true in Hxbound.
+      apply bool_decide_eq_true in Hybound.
+      apply bool_decide_eq_false in Hyx.
+      assert (Hyxbound : bool_decide (y - x ≤ Message2') = true).
+      { apply bool_decide_eq_true. lia. }
+      rewrite Hyxbound; apply bool_decide_eq_true in Hyxbound.
+      assert (Hybound' : bool_decide (y < y - x) = false) by
+        (apply bool_decide_eq_false; lia).
+      rewrite Hybound'. lia.
+  Qed.
+      
+
+
+  Lemma xor_minus_mod_sem_bij x: Bij (xor_minus_mod_sem x).
+  Proof. split.
+    - rewrite /Inj. intros y y'.
+      rewrite /xor_minus_mod_sem.
+      destruct (bool_decide (0 ≤ x)) eqn:Hxpos; simpl; last done.
+      destruct (bool_decide (0 ≤ y)) eqn:Hypos; simpl;
+      destruct (bool_decide (x ≤ Output2')) eqn:Hxbound; try done.
+      destruct (bool_decide (y ≤ Output2')) eqn:Hy'bound; simpl;
+      destruct (bool_decide (y' ≤ Output2')) eqn:Hybound; simpl; try done;
+      destruct (bool_decide (y < x)) eqn:Hyx; simpl;
+      try apply bool_decide_eq_true in Hxpos;
+      try apply bool_decide_eq_true in Hypos;
+      try apply bool_decide_eq_true in Hxbound;
+      try apply bool_decide_eq_true in Hybound;
+      try apply bool_decide_eq_true in Hy'bound;
+      try apply bool_decide_eq_true in Hyx;
+      try apply bool_decide_eq_false in Hxpos;
+      try apply bool_decide_eq_false in Hypos;
+      try apply bool_decide_eq_false in Hxbound;
+      try apply bool_decide_eq_false in Hybound;
+      try apply bool_decide_eq_false in Hy'bound;
+      try apply bool_decide_eq_false in Hyx;
+      try (intros H; exfalso; lia);
+      destruct (bool_decide (y' < x)) eqn:Hy'x; simpl;
+      try apply bool_decide_eq_true in Hy'x;
+      try apply bool_decide_eq_false in Hy'x;
+      try (intros H; lia).
+    - intros y.
+      destruct (bool_decide (0 ≤ x)) eqn:Hxpos; simpl;
+      destruct (bool_decide (x ≤ Output2')) eqn:Hxbound; simpl;
+      try (exists y; rewrite /xor_minus_mod_sem;
+        rewrite Hxpos Hxbound; simpl; reflexivity).
+      destruct (bool_decide (0 ≤ y)) eqn:Hypos; simpl;
+      destruct (bool_decide (y ≤ Output2')) eqn:Hybound; simpl;
+      try (exists y; rewrite /xor_minus_mod_sem;
+        rewrite Hxpos Hxbound Hypos Hybound; simpl; reflexivity).
+      destruct (bool_decide (y + x ≤ Message2')) eqn:Hyplusxbound.
+      * exists (y+x). rewrite /xor_minus_mod_sem.
+        rewrite Hxpos Hxbound Hyplusxbound; simpl.
+        assert (Hyxx : bool_decide (y + x < x) = false)
+          by (apply bool_decide_eq_false; lia).
+        rewrite Hyxx. lia.
+      * exists (y+x - Output2).
+        rewrite /xor_minus_mod_sem.
+        rewrite Hxpos Hxbound; simpl.
+        apply bool_decide_eq_true in Hxpos;
+        apply bool_decide_eq_true in Hypos;
+        apply bool_decide_eq_true in Hxbound;
+        apply bool_decide_eq_true in Hybound;
+        apply bool_decide_eq_false in Hyplusxbound.
+        assert (Hargbound : bool_decide (y + x - Output2 ≤ Message2') = true)
+          by (apply bool_decide_eq_true; lia).
+        rewrite Hargbound.
+        assert (Hargx : bool_decide (y + x - Output2 < x) = true)
+          by (apply bool_decide_eq_true; lia).
+        rewrite Hargx. lia.
+  Qed.
+  
+  Lemma xor_minus_mod_sem_dom: forall x, x < S Message2' -> (∀ n : nat, n < S Output2' →  (xor_minus_mod_sem x n) < S Output2').
+  Proof.
+    intros.
+    rewrite /xor_minus_mod_sem.
+    case_bool_decide;
+    last case_bool_decide;
+    try case_bool_decide; simpl; try lia.
+    case_bool_decide; simpl; try case_bool_decide; try lia.
+  Qed.
+
+  Lemma xor_minus_mod_correct_l `{!approxisRGS Σ} E K (x : Z) (y : nat)
+    (_: (0<=x)%Z)
+    (Hx : ((Z.to_nat x) < S Message2'))
+    (Hy : y < S Message2' ) e A:
+    (REL (fill K (of_val #(xor_minus_mod_sem (Z.to_nat x) (y)))) << e @ E : A)
+    -∗ REL (fill K (xor_minus_mod #x #y)) << e @ E : A.
+  Proof with rel_pures_l.
+    iIntros "H".
+    rewrite /xor_minus_mod...
+    rewrite /Output2' in Hx.
+    rewrite /Output2' in Hy.
+    rewrite /xor_minus_mod_sem.
+    assert (Hxpos : bool_decide (0 ≤ Z.to_nat x) = true);
+    assert (Hypos : bool_decide (0 ≤ y) = true);
+    assert (Hxbound : bool_decide (Z.to_nat x ≤ Message2') = true);
+    assert (Hybound : bool_decide (y ≤ Message2') = true); try apply bool_decide_eq_true;
+    try rewrite /Message2'; try lia.
+    rewrite Hxpos Hypos Hxbound Hybound. simpl.
+    destruct (bool_decide (y < Z.to_nat x)) eqn:Hyx.
+    - assert (Hyx' : bool_decide (y < x)%Z = true) by
+        (apply bool_decide_eq_true; apply bool_decide_eq_true in Hyx; lia).
+        rewrite Hyx'...
+        replace (y - x + S (2 ^ bit - 1))%Z with 
+          (Z.of_nat (S (2 ^ bit - 1 + y) - Z.to_nat x)) by lia.
+        rel_apply "H".
+    - assert (Hyx' : bool_decide (y < x)%Z = false) by
+        (apply bool_decide_eq_false; apply bool_decide_eq_false in Hyx; lia).
+        rewrite Hyx'...
+        replace (y - x)%Z with 
+          (Z.of_nat (y - Z.to_nat x)); first rel_apply "H".
+        apply bool_decide_eq_true in Hypos.
+        apply bool_decide_eq_true in Hxbound.
+        apply bool_decide_eq_true in Hybound.
+        apply bool_decide_eq_false in Hyx.
+        apply bool_decide_eq_false in Hyx'.
+        lia.
+  Qed.
+
+  Lemma xor_minus_mod_correct_r  `{!approxisRGS Σ} E K (x : Z) (y : nat)
+    (_: (0<=x)%Z)
+    (Hx : ((Z.to_nat x) < S Message2'))
+    (Hy: y < S Message2') e A:
+    (REL e << (fill K (of_val #(xor_minus_mod_sem (Z.to_nat x) (y)))) @ E : A)
+    -∗ REL e << (fill K (xor_minus_mod #x #y)) @ E : A.
+  Proof with rel_pures_r.
+    iIntros "H".
+    rewrite /xor_minus_mod...
+    rewrite /Output2' in Hx.
+    rewrite /Output2' in Hy.
+    rewrite /xor_minus_mod_sem.
+    assert (Hxpos : bool_decide (0 ≤ Z.to_nat x) = true);
+    assert (Hypos : bool_decide (0 ≤ y) = true);
+    assert (Hxbound : bool_decide (Z.to_nat x ≤ Message2') = true);
+    assert (Hybound : bool_decide (y ≤ Message2') = true); try apply bool_decide_eq_true;
+    try rewrite /Message2'; try lia.
+    rewrite Hxpos Hypos Hxbound Hybound. simpl.
+    destruct (bool_decide (y < Z.to_nat x)) eqn:Hyx.
+    - assert (Hyx' : bool_decide (y < x)%Z = true) by
+        (apply bool_decide_eq_true; apply bool_decide_eq_true in Hyx; lia).
+        rewrite Hyx'...
+        replace (y - x + S (2 ^ bit - 1))%Z with 
+          (Z.of_nat (S (2 ^ bit - 1 + y) - Z.to_nat x)) by lia.
+        rel_apply "H".
+    - assert (Hyx' : bool_decide (y < x)%Z = false) by
+        (apply bool_decide_eq_false; apply bool_decide_eq_false in Hyx; lia).
+        rewrite Hyx'...
+        replace (y - x)%Z with 
+          (Z.of_nat (y - Z.to_nat x)); first rel_apply "H".
+        apply bool_decide_eq_true in Hypos.
+        apply bool_decide_eq_true in Hxbound.
+        apply bool_decide_eq_true in Hybound.
+        apply bool_decide_eq_false in Hyx.
+        apply bool_decide_eq_false in Hyx'.
+        lia.
+  Qed.
+
+  #[local] Instance XOR_minus_mod : @XOR Output2' Output2'.
+  Proof.
+    unshelve econstructor.
+    2: exact xor_minus_mod.
+    1: exact xor_minus_mod_sem.
+    1: exact xor_minus_mod_sem_bij.
+    apply xor_minus_mod_sem_dom.
+  Defined.
+
+  Fact xor_minus_mod_sem_typed : forall `{!approxisRGS Σ},
+      ⊢ (lrel_int_bounded 0 Key2' → lrel_int_bounded 0 Input2' → lrel_int_bounded 0 Output2')%lrel
+          xor_minus_mod xor_minus_mod.
+  Proof with (rel_pures_r ; rel_pures_l).
+    intros *. rel_vals.
+    iIntros (v1 v2 [x [eq1 [eq2 [Hxpos Hxbound]]]]); subst...
+    rewrite /xor_minus_mod...
+    rel_arrow_val.
+    iIntros (v1 v2 [y [eq1 [eq2 [Hypos Hybound]]]]); subst...
+    case_bool_decide as Hyminusx; rel_pures_l; rel_pures_r; rel_vals;
+      rewrite /Message2'; rewrite /Key2' in Hxbound; rewrite /Input2' in Hybound;
+      lia.
+  Qed.
+
+  #[local] Instance XOR_spec_minus_mod `{!approxisRGS Σ} : @XOR_spec _ _ Output2' Output2' XOR_minus_mod.
+  Proof.
+    unshelve econstructor.
+    - intros. eapply xor_minus_mod_correct_l => //.
+    - intros. eapply xor_minus_mod_correct_r => //.
+    - intros. simpl. eapply xor_minus_mod_sem_typed.
+    - apply xor_minus_mod_sem_inverse_r.
+  Qed.
+
+End xor_minus_mod.
+ 
